theories/Syntax.v
@@ -72,7 +72,7 @@ Section DecEqTerms.
 
   Lemma eqb_term_eq :
     forall t u : Term_ func var, eqb_term t u = true <-> t = u.
-  Proof.
+  Proof using Type.
     intros t; induction t as [n | x | f xs IHxs] using term_rect';
       intro u; destruct u as [m | y | g ys]; split; cbn.
     all: try (now intro).
@@ -80,9 +80,15 @@ Section DecEqTerms.
     - intro e. injection e => ->. rewrite eqbIsEq //.
     - rewrite eqbIsEq. now intros ->.
     - intros e; injection e => ->. rewrite eqbIsEq //.
-    - admit. (* easy, todo *)
-    - intros e; injection e => -> ->. admit. (* easy *)
-  Admitted.
+    - intros (e & e')%andb_prop. rewrite eqbIsEq in e. rewrite e.
+      apply f_equal. eapply forallb2_eq; eauto.
+      intros. rewrite -IHxs; auto.
+    - intros e; injection e => -> ->.
+      rewrite Bool.andb_true_iff. split.
+      + apply EqBool_refl.
+      + apply forallb2_refl. intros. rewrite IHxs; auto.
+        now injection e => -> _.
+  Qed.
 
   #[global] Instance EqBool_term : EqBool (Term_ func var).
   Proof.
@@ -348,189 +354,4 @@ Module ConcreteSyntaxInstances.
 
   Definition Term := Term_ string string.
   Definition Form := Form_ string string string.
-
-  (** *** Set of [Term]s. *)
-  Module OrderedTerm <: SimpleOrderedType.
-    Definition t := Term.
-
-    Inductive lt_list {A : Type} {lt : A -> A -> Prop} : list A -> list A -> Prop :=
-    | lt_head : forall (t u : A) (l l' : list A), lt t u -> lt_list (t :: l) (u :: l')
-    | lt_cons : forall (t : A) (l l' : list A), lt_list l l' -> lt_list (t :: l) (t :: l').
-    Arguments lt_list {_} _ _ _.
-
-    Lemma lt_list_irrefl :
-      forall {A : Type} {lt : A -> A -> Prop} (l : list A),
-        (forall t, In t l -> lt t t -> False) -> lt_list lt l l -> False.
-    Proof.
-      intros A lt l hirrefl hlt.
-      have H0 : exists l', lt_list lt l l' /\ l = l' by exists l.
-      destruct H0 as (l' & H' & e); induction H'.
-      - injection e => e0 e1; subst. unshelve eapply hirrefl.
-        + exact u.
-        + now right.
-        + assumption.
-      - injection e => e0; subst. apply IHH'; auto.
-        intros; eapply hirrefl; eauto. now left.
-    Qed.
-
-    Fixpoint compare_list {A : Type} (cmp : A -> A -> comparison) (l l' : list A) : comparison :=
-      match l, l' with
-      | [], [] => Eq
-      | [], _  => Lt
-      | _ , [] => Gt
-      | x :: xs, y :: ys =>
-          match cmp x y with
-          | Eq => compare_list cmp xs ys
-          | _ as v => v
-          end
-      end.
-
-    Inductive lt_ : Term -> Term -> Prop :=
-    | termLtBoundBound : forall (n m : nat), n < m -> lt_ (Bound n) (Bound m)
-    | termLtBoundFree  : forall (n : nat) (x : string), lt_ (Bound n) (Free x)
-    | termLtBoundFun   : forall (n : nat) (f : string) (l : list Term), lt_ (Bound n) (Fun f l)
-    | termLtFreeFree   : forall (x y : string), OrderedString.lt x y -> lt_ (Free x) (Free y)
-    | termLtFreeFun    : forall (x : string) (f : string) (l : list Term), lt_ (Free x) (Fun f l)
-    | termLtFunFun1    : forall (f f' : string) (l l' : list Term),
-        OrderedString.lt f f' -> lt_ (Fun f l) (Fun f' l')
-    | termLtFunFun2    : forall (f : string) (l l' : list Term),
-        lt_list lt_ l l' -> lt_ (Fun f l) (Fun f l').
-
-    (* Definition lt_ind' (P : Term -> Term -> Prop) (f : forall n m : nat, n < m -> P (Bound n) (Bound m)) *)
-    (*   (f0 : forall (n : nat) (x : string), P (Bound n) (Free x)) *)
-    (*   (f1 : forall (n : nat) (f1 : string) (l : list Term), P (Bound n) (Fun f1 l)) *)
-    (*   (f2 : forall x y : string, OrderedString.lt x y -> P (Free x) (Free y)) *)
-    (*   (f3 : forall (x f3 : string) (l : list Term), P (Free x) (Fun f3 l)) *)
-    (*   (f4 : forall (f4 f' : string) (l l' : list Term), OrderedString.lt f4 f' -> P (Fun f4 l) (Fun f' l')) *)
-    (*   (f5 : forall (f5 : string) (l l' : list Term), *)
-    (*       (forall i t u, nth_error l i = Some t -> nth_error l' i = Some u -> lt t u -> P t u) -> *)
-    (*       lt_list lt l l' -> P (Fun f5 l) (Fun f5 l')) *)
-    (*    : forall (t t0 : Term), lt t t0 -> P t t0. *)
-    (* Proof. *)
-    (*   refine (fix F (t t0 : Term) (h : lt t t0) : P t t0 := *)
-    (*             let fix F_list (l l' : list Term) (h0 : lt_list lt l l') : *)
-    (*               (forall i t u, nth_error l i = Some t -> nth_error l' i = Some u -> lt t u -> P t u) := _ *)
-    (*             in *)
-    (*             match h in (lt t1 t2) return (P t1 t2) with *)
-    (*             | termLtBoundBound n m x => f n m x *)
-    (*             | termLtBoundFree n x => f0 n x *)
-    (*             | termLtBoundFun n f6 l0 => f1 n f6 l0 *)
-    (*             | termLtFreeFree x y x0 => f2 x y x0 *)
-    (*             | termLtFreeFun x f6 l0 => f3 x f6 l0 *)
-    (*             | termLtFunFun1 f6 f' l0 l' x => f4 f6 f' l0 l' x *)
-    (*             | termLtFunFun2 f6 l0 l' x => f5 f6 l0 l' (F_list l0 l' x) x *)
-    (*             end). *)
-    (*   intros. destruct h0. *)
-    (*   - now apply F. *)
-    (*   - destruct i; cbn in *. *)
-    (*     + now apply F. *)
-    (*     + eapply F_list; eauto. *)
-    (* Defined. *)
-
-    Definition lt := lt_.
-
-    Lemma lt_strorder : StrictOrder lt.
-    Proof. Admitted.
-    (* split. *)
-    (* - intros t H. *)
-    (*   have H0 : exists u, lt t u /\ t = u by exists t. *)
-    (*   destruct H0 as (u & H' & e); induction H'; *)
-    (*     try (inversion e; fail). *)
-    (*   + injection e => e'. rewrite e' in H0. *)
-    (*     now apply StrictOrder_Irreflexive in H0. *)
-    (*   + injection e => e'. rewrite e' in H0. *)
-    (*     now apply StrictOrder_Irreflexive in H0. *)
-    (*   + injection e => _ e'. rewrite e' in H0. *)
-    (*     now apply StrictOrder_Irreflexive in H0. *)
-    (*   + injection e => e'; subst. eapply lt_list_irrefl. *)
-    (*     2: exact H0. *)
-
-    (*     intros. *)
-    (*   apply H. intros l hlt. *)
-    (*   have H0 : exists l', lt_list l l' /\ l = l' by exists l. *)
-    (*   destruct H0 as (l' & H' & e); induction H'. *)
-    (*   + injection e => e0 e1; subst. *)
-    (*     have contra : (lt u u -> False). *)
-    (*     { apply H. intro. intro. *)
-    (*     injection e' => _ e0. subst. apply IHH'; auto. *)
-    (* - intros t u v htu huv. *)
-    (*   have H0 : exists u', lt u' v /\ u = u' by exists u. *)
-    (*   destruct H0 as (u' & H' & e). clear huv. induction htu; destruct H'. *)
-    (*   (** trivial cases *) *)
-    (*   all: try now constructor. *)
-    (*   (** inconsistency in the equality *) *)
-    (*   all: try (inversion e; fail). *)
-    (*   + constructor. eapply StrictOrder_Transitive; eauto. *)
-    (*     injection e => e'; now subst. *)
-    (*   + constructor. eapply StrictOrder_Transitive; eauto. *)
-    (*     injection e => e'; now subst. *)
-    (*   + injection e => e' e''; subst. constructor. *)
-    (*     eapply StrictOrder_Transitive; eauto. *)
-    (*   + injection e => e' e''; subst; now constructor. *)
-    (*   + injection e => e' e''; subst; now constructor. *)
-    (*   + injection e => e' e''. rewrite e''. *)
-    (*     have H : lt t0 u0. *)
-    (*     {  *)
-    (*     eapply termLtFunFun2. *)
-
-    Lemma lt_compat : Proper (Logic.eq ==> Logic.eq ==> iff) lt.
-    Proof.
-      intros t u e t' u' e'. split.
-      + intros; now subst.
-      + intros; now subst.
-    Qed.
-
-    Fixpoint compare (t u : Term) : comparison :=
-      match t, u with
-      | Bound n, Bound m => OrderedNat.compare n m
-      | Bound _, Free  _ => Lt
-      | Bound _, Fun _ _ => Lt
-      | Free _ , Bound _ => Gt
-      | Free x , Free y  => OrderedString.compare x y
-      | Free _ , Fun _ _ => Lt
-      | Fun _ _, Bound _ => Gt
-      | Fun _ _, Free _ => Gt
-      | Fun x xs, Fun y ys =>
-          match OrderedString.compare x y with
-          | Eq => compare_list compare xs ys
-          | _ as v => v
-          end
-      end.
-
-    Lemma compare_spec :
-      forall t u : Term, CompareSpec (t = u) (lt t u) (lt u t) (compare t u).
-    Proof.
-      intros t u; destruct t, u; cbn.
-      - destruct (OrderedNat.compare n n0) eqn:e.
-        + constructor.
-          apply PeanoNat.Nat.compare_eq in e; now subst.
-        + constructor.
-          apply PeanoNat.Nat.compare_lt_iff in e. now constructor.
-        + constructor.
-          apply PeanoNat.Nat.compare_gt_iff in e. now constructor.
-      - do 2 constructor.
-      - do 2 constructor.
-      - do 2 constructor.
-      - have H := (OrderedString.compare_spec a a0); destruct H.
-        + constructor. now rewrite H.
-        + now do 2 constructor.
-        + now do 2 constructor.
-      - do 2 constructor.
-      - do 2 constructor.
-      - do 2 constructor.
-      - have H := (OrderedString.compare_spec a a0); destruct H.
-        + generalize dependent l0. induction l; destruct l0.
-          * constructor. now rewrite H.
-          * constructor. admit.
-          * constructor. admit.
-          * admit.
-        + now do 2 constructor.
-        + now do 2 constructor.
-    Admitted.
-
-    Definition eq_bool : EqBool Term := ltac:(typeclasses eauto).
-  End OrderedTerm.
-
-  Module SetOfTerm_ := SetFromOrdered OrderedTerm.
-  Canonical Structure SetOfTerm := SetOfTerm_.set_of_ordered.
 End ConcreteSyntaxInstances.
